fixing some naming and adding tex

MealyMachine.thy
@@ -4,72 +4,80 @@ begin
 
 sledgehammer_params [provers = cvc4 verit z3 spass vampire zipperposition]
 
-text \<open>transitions mealy\<close>
-type_synonym ('state,'input,'output) transition = "(('state \<times> 'input) \<Rightarrow> ('state \<times> 'output))"
+text \<open>transs mealy\<close>
+type_synonym ('s,'in,'out) trans = "(('s \<times> 'in) \<Rightarrow> ('s \<times> 'out))"
 
-type_synonym ('state,'input,'output) mealy = "'state \<times> ('state,'input,'output) transition"
-
-
-fun trans_star :: "('state,'input,'output) transition \<Rightarrow> 'state \<Rightarrow> 'input list \<Rightarrow> ('state \<times> 'output list)" where
-"trans_star f q [] = (q, [])" |
-"trans_star f q (w # ws) = (let (st,op) = f (q,w) in (let (q',x) = trans_star f st ws in (q',op # x)))"
+type_synonym ('s,'in,'out) mealy = "'s \<times> ('s,'in,'out) trans"
 
 
-fun trans_star_output :: "('state,'input,'output) transition \<Rightarrow> 'state \<Rightarrow> 'input list \<Rightarrow> ('output list)" where
-"trans_star_output f q [] = []" |
-"trans_star_output f q (i # is) = (let (st,op) = f (q,i) in (let x = trans_star_output f st is in (op # x)))"
+fun run_mealy :: "('s,'in,'out) trans \<Rightarrow> 's \<Rightarrow> 'in list \<Rightarrow> ('s \<times> 'out list)" where
+"run_mealy f q [] = (q, [])" |
+"run_mealy f q (w # ws) = (let (st,op) = f (q,w) in (let (q',x) = run_mealy f st ws in (q',op # x)))"
 
 
-fun trans_star_state :: "('state,'input,'output) transition \<Rightarrow> 'state \<Rightarrow> 'input list \<Rightarrow> ('state)" where
-"trans_star_state f q [] = q" |
-"trans_star_state f q (i # is) = (let (st,op) = f (q,i) in (let x = trans_star_state f st is in x))"
+definition outs_run_mealy :: "('s,'in,'out) trans \<Rightarrow> 's \<Rightarrow> 'in list \<Rightarrow> ('out list)" where
+"outs_run_mealy f q ins =  snd (run_mealy f q ins)" 
 
 
-lemma trans_star_output_state: "trans_star f q i = (trans_star_state f q i,trans_star_output f q i)"
-  apply (induction i arbitrary: f q)
-  apply simp+ 
-  by (smt (verit) case_prod_conv prod.case_distrib split_cong)
+definition state_run_mealy :: "('s,'in,'out) trans \<Rightarrow> 's \<Rightarrow> 'in list \<Rightarrow> ('s)" where
+"state_run_mealy f q ins = fst (run_mealy f q ins)" 
 
-definition mealy_eq :: "('state,'input,'output) mealy \<Rightarrow> 'state \<Rightarrow> ('state2,'input,'output) mealy \<Rightarrow> 'state2 \<Rightarrow> bool" where
-"mealy_eq a q b p \<equiv> (case (a,b) of
-    ((q_0,f),(p_0,g)) \<Rightarrow> (\<forall> is. trans_star_output f q is = trans_star_output g p is))"
 
-abbreviation equal :: "('state,'input,'output) mealy \<Rightarrow> ('state2,'input,'output) mealy \<Rightarrow> bool" (infixr"\<approx>" 80) where
+
+lemma run_mealy_twostep:"run_mealy f q' ins = (q'',out) \<Longrightarrow> f (q,i) = (q',ou) \<Longrightarrow> run_mealy f q (i#ins) = (q'',ou#out)"
+  by simp
+
+lemma outs_run_mealy_twostep:"outs_run_mealy f q' ins = out \<Longrightarrow> f (q,i) = (q',ou) \<Longrightarrow> outs_run_mealy f q (i#ins) = ou#out"
+  unfolding outs_run_mealy_def using run_mealy_twostep 
+  by (metis split_pairs)
+
+lemma out_state_run_mealy: "run_mealy f q i = (state_run_mealy f q i,outs_run_mealy f q i)"
+unfolding outs_run_mealy_def state_run_mealy_def 
+  by auto
+  
+
+definition eq_mealy :: "('s,'in,'out) mealy \<Rightarrow> 's \<Rightarrow> ('s2,'in,'out) mealy \<Rightarrow> 's2 \<Rightarrow> bool" where
+"eq_mealy a q b p \<equiv> (case (a,b) of
+    ((q_0,f),(p_0,g)) \<Rightarrow> (\<forall> is. outs_run_mealy f q is = outs_run_mealy g p is))"
+
+abbreviation equal :: "('s,'in,'out) mealy \<Rightarrow> ('s2,'in,'out) mealy \<Rightarrow> bool" (infixr"\<approx>" 80) where
 "a \<approx> b \<equiv> (case (a,b) of
-    ((q_0,f),(p_0,g)) \<Rightarrow> mealy_eq a q_0 b p_0)"
+    ((q_0,f),(p_0,g)) \<Rightarrow> eq_mealy a q_0 b p_0)"
 
 
 
-definition func_sim :: "('state \<Rightarrow> 'state2) \<Rightarrow> ('state,'input,'output) mealy \<Rightarrow>
-    ('state2,'input,'output) mealy \<Rightarrow> bool" where
-"func_sim f a b \<equiv> (case (a,b) of
+definition func_sim_mealy :: "('s \<Rightarrow> 's2) \<Rightarrow> ('s,'in,'out) mealy \<Rightarrow>
+    ('s2,'in,'out) mealy \<Rightarrow> bool" where
+"func_sim_mealy f a b \<equiv> (case (a,b) of
     ((q_0,t),(p_0,g)) \<Rightarrow> (f q_0 = p_0) \<and> (\<forall> q q' i op. t (q,i) = (q',op) \<longrightarrow>
       g (f q,i) = (f q',op)))"
 
 
-lemma split_trans_star_output: "t (q,i) = (q',ot) \<Longrightarrow> trans_star_output t q' is = op \<Longrightarrow>
-    trans_star_output t q (i # is) = (ot # op)"
+lemma split_outs_run_mealy: "t (q,i) = (q',ot) \<Longrightarrow> outs_run_mealy t q' is = op \<Longrightarrow>
+    outs_run_mealy t q (i # is) = (ot # op)"
+  unfolding outs_run_mealy_def
   by (auto split: prod.splits option.splits)
 
 
-lemma split_trans_star_output_rev: "trans_star_output t q (i # is) = (ot # op) \<Longrightarrow>
-    \<exists> q'. t (q,i) = (q',ot) \<and> trans_star_output t q' is = op"
+lemma split_outs_run_mealy_rev: "outs_run_mealy t q (i # is) = (ot # op) \<Longrightarrow>
+    \<exists> q'. t (q,i) = (q',ot) \<and> outs_run_mealy t q' is = op"
+  unfolding outs_run_mealy_def
   by (auto split: prod.splits option.splits)
 
 
-lemma split_trans_star: "t (q,i) = (q',ot) \<Longrightarrow> trans_star t q' is = (st,op) \<Longrightarrow>
-    trans_star t q (i # is) = (st,ot # op)"
+lemma split_run_mealy: "t (q,i) = (q',ot) \<Longrightarrow> run_mealy t q' is = (st,op) \<Longrightarrow>
+    run_mealy t q (i # is) = (st,ot # op)"
   by (auto split: prod.splits option.splits)
 
 
-lemma split_trans_star_rev: "trans_star t q (i # is) = (st,ot # op) \<Longrightarrow>
-    \<exists> q'. t (q,i) = (q',ot) \<and> trans_star t q' is = (st,op)"
+lemma split_run_mealy_rev: "run_mealy t q (i # is) = (st,ot # op) \<Longrightarrow>
+    \<exists> q'. t (q,i) = (q',ot) \<and> run_mealy t q' is = (st,op)"
   by (auto split: prod.splits option.splits)
 
-lemma trans_star_split_end:
+lemma run_mealy_split_end:
   assumes "t (st,i) = (st',op)" and
-    "trans_star t q acc = (st,out)"
-  shows "trans_star  t q (acc @ [i]) =  (st',out @ [op])"
+    "run_mealy t q acc = (st,out)"
+  shows "run_mealy  t q (acc @ [i]) =  (st',out @ [op])"
 using assms proof (induction acc arbitrary: out q)
   case Nil
   then show ?case 
@@ -79,37 +87,23 @@ next
  
   obtain q' op' where q':"t (q,a) = (q', op')"
     by fastforce
-   then have "trans_star t q (a # acc) = (let (qnew,x) = trans_star t q' acc in (qnew,op' # x)) "
+   then have "run_mealy t q (a # acc) = (let (qnew,x) = run_mealy t q' acc in (qnew,op' # x)) "
      by auto
-   then have "EX outnew. trans_star t q' acc = (st,outnew)" using Cons 
-     by (simp add: trans_star_output_state)
-   then obtain outnew where outnew:"trans_star t q' acc = (st,outnew)" 
+   then have "EX outnew. run_mealy t q' acc = (st,outnew)" using Cons 
+     by (simp add: out_state_run_mealy)
+   then obtain outnew where outnew:"run_mealy t q' acc = (st,outnew)" 
      by presburger
-   then have "trans_star t q' (acc @ [i]) = (st', outnew @ [op])" using Cons 
+   then have "run_mealy t q' (acc @ [i]) = (st', outnew @ [op])" using Cons 
      by blast
-   then have "trans_star t q (a#(acc@[i])) =  (st',op' # outnew@[op]) " using  q' 
+   then have "run_mealy t q (a#(acc@[i])) =  (st',op' # outnew@[op]) " using  q' 
      by simp
   then show ?case using q' outnew 
     using Cons.prems(2) by auto
 qed
 
 
-lemma
-  assumes "trans_star_state t q_0 acc = st" and
-    "trans_star_state t st is = (st2)"
-  shows "(trans_star_state t q_0 (acc @ is)) = (st2)"
-using assms proof (induction t q_0 acc rule: trans_star.induct)
-  case (1 f q)
-  then show ?case
-    by fastforce
-next
-  case (2 f q w ws)
-  then show ?case
-    by (metis (no_types,lifting) append_Cons case_prod_conv old.prod.exhaust trans_star_state.simps(2))
-qed
 
-
-lemma trans_star_length: "trans_star t q_0 iss = (q,os) \<Longrightarrow> length iss = length os"
+lemma run_mealy_length: "run_mealy t q_0 iss = (q,os) \<Longrightarrow> length iss = length os"
 proof (induction iss arbitrary: os q q_0)
   case Nil
   then show ?case
@@ -121,33 +115,33 @@ next
 qed
 
 
-lemma trans_star_two:
-  assumes "trans_star t q_0 acc = (st,op1)" and
-    "trans_star t st is = (st2,op2)"
-  shows "(trans_star t q_0 (acc @ is)) = (st2,op1 @ op2)"
+lemma run_mealy_two:
+  assumes "run_mealy t q_0 acc = (st,op1)" and
+    "run_mealy t st is = (st2,op2)"
+  shows "(run_mealy t q_0 (acc @ is)) = (st2,op1 @ op2)"
 using assms proof (induction acc arbitrary: q_0 op1 op2 st st2)
   case Nil
   then show ?case
     by fastforce
 next
   case (Cons w ws)
-  have a: "trans_star_output t q_0 (w # ws) = op1"
-    using trans_star_output_state Cons
+  have a: "outs_run_mealy t q_0 (w # ws) = op1"
+    using out_state_run_mealy Cons
     by (metis prod.inject)
   then obtain op11 op12 where
     op: "op1 = op11 # op12"
-    by (meson old.prod.exhaust split_trans_star_output)
-  then have "\<exists> q'. t (q_0,w) = (q',op11) \<and> trans_star t q' ws = (st,op12)"
-    using split_trans_star_rev Cons
+    by (meson old.prod.exhaust split_outs_run_mealy)
+  then have "\<exists> q'. t (q_0,w) = (q',op11) \<and> run_mealy t q' ws = (st,op12)"
+    using split_run_mealy_rev Cons
     by fast
   then obtain q' where
-    q': "t (q_0,w) = (q',op11) \<and> trans_star t q' ws = (st,op12)"
+    q': "t (q_0,w) = (q',op11) \<and> run_mealy t q' ws = (st,op12)"
     by blast
-  then have "trans_star t q' (ws @ is) = (st2,op12 @ op2)"
+  then have "run_mealy t q' (ws @ is) = (st2,op12 @ op2)"
     using Cons
     by blast
-  then have "trans_star t q_0 (w # ws @ is) = (st2,op11 # op12 @ op2)"
-    using split_trans_star q'
+  then have "run_mealy t q_0 (w # ws @ is) = (st2,op11 # op12 @ op2)"
+    using split_run_mealy q'
     by simp
   then show ?case
     by (simp add: op)
@@ -155,34 +149,34 @@ next
 qed
 
 
-lemma trans_star_two_nested:
-"trans_star t (fst (trans_star t q_0 acc)) is =
-    (fst (trans_star t q_0 (acc @ is)),drop (length acc) (snd (trans_star t q_0 (acc @ is))))"
+lemma run_mealy_two_nested:
+"run_mealy t (fst (run_mealy t q_0 acc)) is =
+    (fst (run_mealy t q_0 (acc @ is)),drop (length acc) (snd (run_mealy t q_0 (acc @ is))))"
 proof -
   obtain st op1 where
-    op1: "(trans_star t q_0 acc) = (st,op1)"
+    op1: "(run_mealy t q_0 acc) = (st,op1)"
     by fastforce
   obtain st2 op2 where
-    op2: "(trans_star t st is) = (st2,op2)"
+    op2: "(run_mealy t st is) = (st2,op2)"
     by fastforce
-  have "trans_star t (fst (trans_star t q_0 acc)) is = trans_star t st is"
+  have "run_mealy t (fst (run_mealy t q_0 acc)) is = run_mealy t st is"
     using op1 op2
     by simp
   show ?thesis proof (standard,goal_cases)
     case 1
-    have "fst (trans_star t q_0 (acc @ is)) = fst (trans_star t st is)"
-      using trans_star_two op1 op2
+    have "fst (run_mealy t q_0 (acc @ is)) = fst (run_mealy t st is)"
+      using run_mealy_two op1 op2
       by fastforce
     then show ?case
       using op1 op2
       by auto
   next
     case 2
-    have a: "snd (trans_star t q_0 (acc @ is)) = (op1 @ op2)"
-      using op1 op2 trans_star_two
+    have a: "snd (run_mealy t q_0 (acc @ is)) = (op1 @ op2)"
+      using op1 op2 run_mealy_two
       by fastforce
     have "length op1 = length acc"
-      using op1 trans_star_length
+      using op1 run_mealy_length
       by metis
     then have "drop (length acc) (op1 @ op2) = op2"
       by simp
@@ -194,18 +188,19 @@ qed
 
 
 lemma sim_subset:
-  assumes "func_sim f (q_0,t) (p_0,g)" and
-    "trans_star_output t q i = ot"
-  shows "trans_star_output g (f q) i = ot"
+  assumes "func_sim_mealy f (q_0,t) (p_0,g)" and
+    "outs_run_mealy t q i = ot"
+  shows "outs_run_mealy g (f q) i = ot"
 using assms proof (induction i arbitrary: q ot)
   case Nil
   then show ?case
+     unfolding outs_run_mealy_def
     by fastforce
 next
   case (Cons a i)
   have a: "\<forall> q' ot. t (q,a) = (q',ot) \<longrightarrow> g (f q,a) = (f q',ot)"
     using assms Cons
-    unfolding func_sim_def
+    unfolding func_sim_mealy_def
     by simp     
   have "\<exists> q' out. t (q,a) = (q',out)"
     using Cons
@@ -215,16 +210,16 @@ next
     using Cons
     by fastforce
   then have "\<exists> os. ot = out # os"
-    using Cons
+    using Cons   unfolding outs_run_mealy_def
     by (auto split: prod.splits option.splits)
   then obtain os where
     ot: "ot = out # os"
     by auto
-  then have "trans_star_output t q' i = os \<Longrightarrow> trans_star_output g (f q') i = os"
+  then have "outs_run_mealy t q' i = os \<Longrightarrow> outs_run_mealy g (f q') i = os"
     using Cons assms 
     by blast
-  then have "trans_star_output t q (a # i) = (out # os) \<Longrightarrow> trans_star_output g (f q) (a # i) = (out # os)"
-    using a q split_trans_star_output
+  then have "outs_run_mealy t q (a # i) = (out # os) \<Longrightarrow> outs_run_mealy g (f q) (a # i) = (out # os)"
+    using a q split_outs_run_mealy   unfolding outs_run_mealy_def
     by (auto split: prod.splits option.splits)
   then show ?case
     using Cons q a ot
@@ -232,39 +227,35 @@ next
 qed
 
 
-definition apart :: "('state,'input,'output) mealy \<Rightarrow> 'state \<Rightarrow> 'state \<Rightarrow> bool" where
-"apart m q p \<equiv> (case m of
-    (q_0,t) \<Rightarrow> \<exists> i x y. trans_star_output t p i = x \<and> trans_star_output t q i = y \<and> x \<noteq> y)"
+definition apart_mealy :: "('s,'in,'out) mealy \<Rightarrow> 's \<Rightarrow> 's \<Rightarrow> bool" where
+"apart_mealy m q p \<equiv> (case m of
+    (q_0,t) \<Rightarrow> \<exists> i x y. outs_run_mealy t p i = x \<and> outs_run_mealy t q i = y \<and> x \<noteq> y)"
 
 
-definition apart_with_witness :: "('state,'input,'output) mealy \<Rightarrow> 'state \<Rightarrow> 'state \<Rightarrow> 'input list \<Rightarrow> bool" where
-"apart_with_witness m q p is \<equiv> (case m of
-    (q_0,t) \<Rightarrow> \<exists> x y. trans_star_output t p is = x \<and> trans_star_output t q is = y \<and> x \<noteq> y)"
-
-fun apart_machines :: "('state,'input,'output) transition \<Rightarrow> 'state \<Rightarrow> ('state2,'input,'output) transition \<Rightarrow> 'state2 \<Rightarrow> bool" where
-"apart_machines t q f p = (\<exists> i. trans_star_output t q i \<noteq> trans_star_output f p i)"
+fun apart_machines :: "('s,'in,'out) trans \<Rightarrow> 's \<Rightarrow> ('s2,'in,'out) trans \<Rightarrow> 's2 \<Rightarrow> bool" where
+"apart_machines t q f p = (\<exists> i. outs_run_mealy t q i \<noteq> outs_run_mealy f p i)"
 
 lemma simulation_apart:
-  assumes "func_sim f (q_0,t) (p_0,g)" and
-    "apart (q_0,t) q q'" 
-  shows "\<not> mealy_eq (p_0,g) (f q) (p_0,g) (f q')"
+  assumes "func_sim_mealy f (q_0,t) (p_0,g)" and
+    "apart_mealy (q_0,t) q q'" 
+  shows "\<not> eq_mealy (p_0,g) (f q) (p_0,g) (f q')"
 proof
-  assume "mealy_eq (p_0,g) (f q) (p_0,g) (f q')"
-  then have c: "(\<forall> is. trans_star_output g (f q) is = trans_star_output g (f q') is)"
-    unfolding mealy_eq_def
+  assume "eq_mealy (p_0,g) (f q) (p_0,g) (f q')"
+  then have c: "(\<forall> is. outs_run_mealy g (f q) is = outs_run_mealy g (f q') is)"
+    unfolding eq_mealy_def
     by fastforce
-  have "\<exists> w x y. trans_star_output t q w = x \<and> trans_star_output t q' w = y \<and> x \<noteq> y"
+  have "\<exists> w x y. outs_run_mealy t q w = x \<and> outs_run_mealy t q' w = y \<and> x \<noteq> y"
     using assms (2)
-    unfolding apart_def
+    unfolding apart_mealy_def
     apply simp
     by metis
   then obtain w x y where
-    w: "trans_star_output t q w = x \<and> trans_star_output t q' w = y \<and> x \<noteq> y"
+    w: "outs_run_mealy t q w = x \<and> outs_run_mealy t q' w = y \<and> x \<noteq> y"
     by blast
-  then have a: "trans_star_output g (f q) w = x"
+  then have a: "outs_run_mealy g (f q) w = x"
     using assms sim_subset
     by fast
-  have b: "trans_star_output g (f q') w = y"
+  have b: "outs_run_mealy g (f q') w = y"
     using w assms sim_subset
     by meson
   have d: "x \<noteq> y"
